\documentclass[12pt]{article}
\usepackage{amsmath, amssymb, amsthm, amsfonts, geometry}
\newtheorem{theorem}{Theorem}
\newtheorem{lemma}{Lemma}
\newtheorem{proposition}{Proposition}
\newtheorem{corollary}{Corollary}
\newtheorem{definition}{Definition}

% Page Setup
\geometry{top=1in, bottom=1in, left=1in, right=1in}

\title{Lecture Notes: Abstract Algebra | Internal Direct Products (Course By: Alvaro Lozano-Robledo)}
\author{Thobias K. HÃ¸ivik}
\date{\today}

\begin{document}

\maketitle
\noindent
The goal is to see if a group G is isomorphic to subgroups of G, 
i.e \(G \cong H \times K, H,K \leq G\).

\noindent
\textbf{Example:}

\noindent 
\(U(8) = (\mathbb Z /_8 \mathbb Z)^\times = \{1,3,5,7 \text{ mod } 8\}\)

\noindent 
\(
    U(8) \cong \mathbb Z/_2 \mathbb Z \times 
    \mathbb Z /_2 \mathbb Z
\)

\noindent 
\begin{proposition}
    Let \(H = \{1,3\} = <3>, K = \{1,5\} = <5>\). 
    Then \(\phi: H\times K \to U(8)\) given by 
    \((h,k) \to h \cdot k\) with the domain- and codomain elements 
    taken mod 8 is a bijection, making \(U(8) \cong H\times K\). 
\end{proposition}

\begin{proof}
    Let \(H = \{1,3\}, K = \{1,5\}\).
    Bijection: 
    \begin{gather*}
        (1,1) \to 1 \\ 
        (3,1) \to 3 \\ 
        (1,5) \to 5 \\ 
        (3,5) \to 3 \cdot 5 \equiv 15 \equiv 7 \text{ mod } 8
    \end{gather*}
    Homomorphism:
    \begin{gather*}
        \phi((h,k) \cdot (a, b)) = \phi(ha, kb) \\ 
        = h\cdot a \cdot k \cdot b = hk \cdot ab \\ 
        = \phi(h,k) \cdot \phi(a,b)
    \end{gather*}
    Thus, \(U(8) \cong H \times K\) isomorphic to the direct 
    product of two subgroups of \(U(8)\).
\end{proof}

\break 
\begin{proposition}
    Let G be a group, and let \(H,K \leq G\) subgroups such that: 
    \begin{enumerate}
        \item \(G = H\cdot K = \{h\cdot k : h\in H, k \in K\}\)
        \item \(H \cap K = \{e\}\)
        \item \(hk = kh,\) \(\forall h \in H, k \in K\)
    \end{enumerate}
    Then G is isomorphic to \(H \times K\) via 
    \begin{gather*}
        \phi: H \times K \to G \\ 
        (h,k) \to h \cdot k
    \end{gather*}
    If so we say that G is internal direct product of H and K.

\end{proposition}

\begin{proof}
    \(\phi: H \times K \to G, (h,k) \to h \cdot k\). 
    The map is well defined, 
    \[
        h \in H \subseteq G \land k \in K \subseteq G 
        \Rightarrow h\star k \in G
    \]
    Injective: 
    \[ 
        \phi(h,k) = \phi(a,b) \Rightarrow 
        h \cdot k = a \cdot b 
    \]
    \[ 
        \Rightarrow a^{-1}h = bk^{-1} \in H \cap K = \{e\} 
    \]
    \[ 
        \Rightarrow a = h \land b = k, \text{ } 
        \therefore \boxed{(h,k) = (a,b)}
    \]
    Surjective: 
    
    \noindent  
    By assumption \(HK = G\), so \(\exists h\in H \land \exists k 
    \in K\) such that \(hk = g \in G\).

    \noindent 
    Homomorphism: 
    \begin{gather*}
        \phi(h,k) \cdot \phi(a,b) = hkab \\ 
        \left( hk=kh, \forall h \in H \land \forall k \in K\right) \\ 
        \Rightarrow hkab = hakb = \phi(ha, kb) 
        = \phi((h,k) \cdot (a,b))
    \end{gather*}
    So \(H\times K \cong G\).
\end{proof}
    


\end{document}
